src/tls/Parsers.Ticket.Low.fsti
@@ -31,19 +31,19 @@ val valid_ticketContents12_intro
     let pos2 = LP.get_valid_pos cipherSuite_parser h input pos1 in
     LP.valid boolean_parser h input pos2 /\ (
     let pos3 = LP.get_valid_pos boolean_parser h input pos2 in
-    LP.valid (LPB.parse_flbytes 48) h input pos3
+    LP.valid ticketContents12_master_secret_parser h input pos3
   )))))
   (ensures (
     let pos1 = LP.get_valid_pos protocolVersion_parser h input pos in
     let pos2 = LP.get_valid_pos cipherSuite_parser h input pos1 in
     let pos3 = LP.get_valid_pos boolean_parser h input pos2 in
-    let pos4 = LP.get_valid_pos (LPB.parse_flbytes 48) h input pos3 in
+    let pos4 = LP.get_valid_pos ticketContents12_master_secret_parser h input pos3 in
     LP.valid_content_pos ticketContents12_parser h input pos
       ({
         pv = LP.contents protocolVersion_parser h input pos;
         Parsers.TicketContents12.cs = LP.contents cipherSuite_parser h input pos1;
         ems = LP.contents boolean_parser h input pos2;
-        master_secret = LP.contents (LPB.parse_flbytes 48) h input pos3;
+        master_secret = LP.contents ticketContents12_master_secret_parser h input pos3;
       })
       pos4
   ))
@@ -130,3 +130,5 @@ val finalize_case_ticketContents13
     /\
     pos' == LP.get_valid_pos ticketContents13_parser h input pos1
   ))
+
+val write_ticketContents12_master_secret : LP.leaf_writer_strong ticketContents12_master_secret_serializer
